- Reorganized of the L6 directory: cps.v now contains the only the syntax of L6, eval.v the semantics, and logical_relations. the two logical relations. - Removed halting continuation application case from the semantics (to be handled as primitive function application) and adapted the relations and the proofs. - Added README.md that describes the L6_PCPS directory.

theories/L6_PCPS/cps.v
@@ -1,20 +1,15 @@
 (* Continuation-Passing Style language for the CertiCoq project.
  *   Initial design, Andrew W. Appel, June 2014
  *)
-Require Import Coq.Relations.Relations.
-Require Import ExtLib.Structures.Monad.
-Require ExtLib.Core.Type.
-Require Import Coq.ZArith.ZArith.
-Require Import Coq.ZArith.Znumtheory.
-Require Import Coq.Bool.Bool.
-Require Import Coq.Lists.List.
+Require Import Coq.Relations.Relations Coq.ZArith.ZArith Coq.ZArith.Znumtheory
+               Coq.Bool.Bool Coq.Lists.List Coq.funind.Recdef.
+Require Import ExtLib.Structures.Monad ExtLib.Core.Type.
 Require Maps.
-Require Coq.funind.Recdef.
 Import Nnat.
+
 Require Import List_util.
-
-
 Require Import HashMap.
+
 
 (* We will use several maps from identifiers to types, values, etc.
  * For now we'll use Xavier Leroy's efficient polymorphic maps from 
@@ -64,23 +59,14 @@ Definition prim := M.elt. (* primitive operators *)
    abstract syntax trees.
  *)
 
-
-Fixpoint mapopt {A} (al: list (option A)) : option (list A) :=
-  match al with 
-    | Some a :: al' => match mapopt al' with
-                         | Some bl' => Some (a::bl')
-                         | None => None
-                       end
-    | None :: _ => None
-    | nil => Some nil
-  end.
-
 (* Given a list of tagged variants, return the one with the matching tag. *)
 Fixpoint findtag {A} (cl: list (tag * A)) (c: tag) : option A :=
   match cl with
     | (c',a)::cl' => if M.elt_eq c' c then Some a else findtag cl' c
     | nil => None
   end.
+
+(** * CPS Expressions *)
 
 (* Expressions [exp] of the CPS language. *)
 Inductive exp : Type :=
@@ -95,6 +81,51 @@ with fundefs : Type :=
      | Fcons: var -> type -> list var -> exp -> fundefs -> fundefs
      | Fnil: fundefs.
 
+
+
+(* [Econstr x t c ys e] applies a data constructor with tag [c] to
+           a list of values denoted by variables [ys].   The resulting
+           value is bound to variable [x] of type [t], and then execution
+           continues with expression [e].  Static typing requires that
+           the typeinfo bound to [t] has a variant consistent with [c]
+           and the types of [ys].
+    [Ecase v cl] does case-discrimination on value [v], which
+           must be a [Vconstr t c vl] value. One of the elements of 
+           [cl] must be the pair [(c,e)], where [e] a expression
+           that uses [v]. 
+           Older approach:  
+           One of the elements of [cl] must be the pair [(c,k)], where
+           [k] is a continuation; this continuation is then applied to
+           the argument [v].  The bound variable of [k] then contains
+           the same value as [v], but with a refined type.
+    [Eproj v t n y e] projects the record value [y] by selecting
+           the [n]th element of the record.   This is bound to [v] of type [t]
+           and execution continues with [e].  Typechecking requires
+           that the type of [y] be a Tdata with a single variant, whose 
+           data list has length at least n.
+    [Efun fl e]  binds the set of mutually recursive functions [fl]
+           into the environment, and continues with [e].
+    [Eapp f ys]   applies the function [f] to arguments [ys]
+    [Eprim x t f ys e] applies primop [f] to arguments [ys]
+            and binds the result to [x] of type [t], continues with [e].
+            The primop [f] is a primitive operator, whose type is equivalent to
+            the CPS transform of [ts->t], where [ts] are the type of the [ys].
+
+   [Fdef f t ys e]   defines a function [f] of type [t] with parameters [ys]
+             and body [e].  We do not syntactically distinguish continuations 
+             from other functions, as Andrew Kennedy does [Compiling with 
+             Continuations, Continued, 2007].  Instead, we rely on the type 
+             system to do it; see below.  This mechanism also permits
+             classifying functions into different calling conventions, even 
+             if they have the same source-language type.
+ *)
+
+(* Remark.  It is conventional in CPS representations to guarantee
+   that no two binding occurrences bind the same variable-name.
+   However, neither the static (typing) semantics nor the dynamic
+   (small-step) semantics requires this.  Some of the transformation
+   (optimization, rewrite) algorithms may require it.
+ *)
 
 (** Induction principles for exp *)
 Lemma exp_ind' :
@@ -208,51 +239,51 @@ Ltac exp_defs_induction IH1 IHl IH2 :=
   | intros ? ? ? ? IH1 ? IH2
   | ].
 
-(* [Econstr x t c ys e] applies a data constructor with tag [c] to
-           a list of values denoted by variables [ys].   The resulting
-           value is bound to variable [x] of type [t], and then execution
-           continues with expression [e].  Static typing requires that
-           the typeinfo bound to [t] has a variant consistent with [c]
-           and the types of [ys].
-    [Ecase v cl] does case-discrimination on value [v], which
-           must be a [Vconstr t c vl] value. One of the elements of 
-           [cl] must be the pair [(c,e)], where [e] a expression
-           that uses [v]. 
-           Older approach:  
-           One of the elements of [cl] must be the pair [(c,k)], where
-           [k] is a continuation; this continuation is then applied to
-           the argument [v].  The bound variable of [k] then contains
-           the same value as [v], but with a refined type.
-    [Eproj v t n y e] projects the record value [y] by selecting
-           the [n]th element of the record.   This is bound to [v] of type [t]
-           and execution continues with [e].  Typechecking requires
-           that the type of [y] be a Tdata with a single variant, whose 
-           data list has length at least n.
-    [Efun fl e]  binds the set of mutually recursive functions [fl]
-           into the environment, and continues with [e].
-    [Eapp f ys]   applies the function [f] to arguments [ys]
-    [Eprim x t f ys e] applies primop [f] to arguments [ys]
-            and binds the result to [x] of type [t], continues with [e].
-            The primop [f] is a primitive operator, whose type is equivalent to
-            the CPS transform of [ts->t], where [ts] are the type of the [ys].
+(** * CPS Values *)
 
-   [Fdef f t ys e]   defines a function [f] of type [t] with parameters [ys]
-             and body [e].  We do not syntactically distinguish continuations 
-             from other functions, as Andrew Kennedy does [Compiling with 
-             Continuations, Continued, 2007].  Instead, we rely on the type 
-             system to do it; see below.  This mechanism also permits
-             classifying functions into different calling conventions, even 
-             if they have the same source-language type.
- *)
+Inductive val : Type :=
+| Vconstr: type -> tag -> list val -> val
+| Vfun: M.t val -> fundefs -> var -> val
+(* Vfun env fds f where 
+       env is the environment at the function binding site
+       fds is the list of mutually recursive functions including f *)
+| Vint: Z -> val.
 
-(* Remark.  It is conventional in CPS representations to guarantee
-   that no two binding occurrences bind the same variable-name.
-   However, neither the static (typing) semantics nor the dynamic
-   (small-step) semantics requires this.  Some of the transformation
-   (optimization, rewrite) algorithms may require it.
- *)
 
-Ltac inv H := inversion H; clear H; subst.
+(** Induction principle for values. *)
+Lemma val_ind' :
+  forall P : val -> Prop,
+    (forall (tau : type) (t : tag), P (Vconstr tau t nil)) ->
+    (forall (tau : type) (t : tag) (v : val) (l : list val),
+       P v -> P (Vconstr tau t l) -> P (Vconstr tau t (v :: l))) ->
+    (forall (t : M.t val) (f0 : fundefs) (v : var), P (Vfun t f0 v)) ->
+    (forall z : Z, P (Vint z)) ->
+    forall v : val, P v.
+Proof.
+  intros P H1 H2 H3 H4.
+  fix 1.
+  destruct v; try (now clear val_ind'; eauto).
+  - induction l as [ | x xs IHxs].
+    eapply H1. eapply H2. apply val_ind'. eauto.
+Qed.
+
+Fixpoint def_funs (fl0 fl: fundefs) (rho0 rho: M.t val) : M.t val :=
+  match fl with
+    | Fcons f t xs e fl' => M.set f (Vfun rho0 fl0 f) (def_funs fl0 fl' rho0 rho)
+    | Fnil => rho
+  end.
+
+Fixpoint find_def (f: var) (fl:  fundefs) :=
+  match fl with
+    | Fcons f' t ys e fl' => if M.elt_eq f f' then Some (t,ys,e)
+                            else find_def f fl'
+    | Fnil => None
+  end.
+
+
+  (** The following are not used anywhere. They have to do either with "well-typedness"
+    * or observable values. We need to go through them to decide if can can through them
+    * away altogether. *)
 
 (*********** static typing ******************)
 Inductive typeinfo : Type :=
@@ -444,11 +475,15 @@ Notation "'let' 'Some' x '<-' c1 ;; c2" :=
 Definition cl_of_casecont (TD: tdict) (Gamma: tenv) (ct: tag*var) 
 : option (tag * list type) :=
   t' <- M.get (snd ct) Gamma ;;
-     f <- TDict.get t' TD ;;
-     match f with Tfun c2 (t2::nil) => d <- TDict.get t2 TD ;;
-                                         match d with (Tdata ((c,t3)::nil)) => ret (fst ct, t3)
-                                                   | _ => None end
-               | _ => None end.
+  f <- TDict.get t' TD ;;
+  match f with
+    | Tfun c2 (t2::nil) =>
+      d <- TDict.get t2 TD ;;
+        match d with
+          | (Tdata ((c,t3)::nil)) => ret (fst ct, t3)
+          | _ => None
+        end
+    | _ => None end.
 
 Fixpoint fundefs_lists (f: fundefs) : (list var * list type * list (list var) * list exp)%type :=
   match f with
@@ -504,765 +539,3 @@ with welltyped_funbodies (TD: tdict): forall (Gamma: tenv) (fbody: fundefs), Pro
                  welltyped TD Gamma' e ->
                  welltyped_funbodies TD Gamma (Fcons f t ys e fbody')
      | WTnil: forall Gamma, welltyped_funbodies TD Gamma Fnil.
-
-
-(*********** evaluation ********************)
-
-Inductive val : Type :=
-| Vconstr: type -> tag -> list val -> val
-| Vfun: M.t val -> fundefs -> var -> val
-(* Vfun env fds f where 
-       env is the environment at the function binding site
-       fds is the list of mutually recursive functions including f *)
-| Vint: Z -> val
-| Vother: type -> val
-(* OSB: add constructor for observer functions *)
-| Vobvs: type -> val
-(* Constructor to return values to the environment. 
- * Note that the values in the list need not be observable. 
- * We could remove it altogether and use Vconstr.
- *)
-| Vobservable : type -> list val -> val.
-
-
-(** Induction principle for values. *)
-Lemma val_ind' :
-  forall P : val -> Prop,
-    (forall (tau : type) (t : tag), P (Vconstr tau t nil)) ->
-    (forall (tau : type) (t : tag) (v : val) (l : list val),
-       P v -> P (Vconstr tau t l) -> P (Vconstr tau t (v :: l))) ->
-    (forall (t : M.t val) (f0 : fundefs) (v : var), P (Vfun t f0 v)) ->
-    (forall z : Z, P (Vint z)) ->
-    (forall t : type, P (Vother t)) ->
-    (forall t : type, P (Vobvs t)) ->
-    (forall (tau : type), P (Vobservable tau nil)) ->
-    (forall (tau : type) (v : val) (l : list val),
-       P v -> P (Vobservable tau l) -> P (Vobservable tau (v :: l))) ->
-    forall v : val, P v.
-Proof.
-  intros P H1 H2 H3 H4 H5 H6 H7 H8.
-  fix 1.
-  destruct v; try (now clear val_ind'; eauto).
-  - induction l as [ | x xs IHxs].
-    eapply H1. eapply H2. apply val_ind'. eauto.
-  - induction l as [ | x xs IHxs].
-    eapply H7. eapply H8. apply val_ind'. eauto.
-Qed.
-
-
-Definition env := M.t val.  (* An [env]ironment maps [var]s to their [val]ues *)
-
-(*
-Inductive type_of_val : val -> type -> Prop :=
-| TVconstr: type_of_val (Vconstr t _ _) t
-| TVfun: type_of_val (?? ) t
-| TVint: type_of_val (Vint _) ?   
-| TVother: type_of_val (Vother t) t
-| TVobvs : type_of_val (Vobs t) t   
-. *)
-
-
-Fixpoint def_funs (fl0 fl: fundefs) (rho0 rho: env) : env :=
-  match fl with
-    | Fcons f t xs e fl' => M.set f (Vfun rho0 fl0 f) (def_funs fl0 fl' rho0 rho)
-    | Fnil => rho
-  end.
-
-Fixpoint find_def (f: var) (fl:  fundefs) :=
-  match fl with
-    | Fcons f' t ys e fl' => if M.elt_eq f f' then Some (t,ys,e)
-                             else find_def f fl'
-    | Fnil => None
-  end.
-
-Definition state := (env*exp)%type.
-
-Definition prims := M.t (list val -> option val).
-
-Section PRIMS.
-
-  Variable pr: prims.  
-
-
-  (* small step semantics *)
-  Inductive step: state -> state -> Prop := 
-  | Step_constr: forall vs rho x t n ys e,
-                   getlist ys rho = Some vs ->
-                   step (rho, Econstr x t n ys e) (M.set x (Vconstr t n vs) rho, e)
-  | Step_proj: forall t' n' vs v rho x t n y e,
-                 M.get y rho = Some (Vconstr t' n' vs) ->
-                 nthN vs n = Some v ->
-                 step (rho, Eproj x t n y e) (M.set x v rho, e)
-  | Step_case: forall t c vl e' rho y cl,
-                 M.get y rho = Some (Vconstr t c vl) ->
-                 findtag cl c = Some e' -> 
-                 step (rho, Ecase y cl) (rho, e')
-  | Step_fun: forall rho fl e,
-                step (rho, Efun fl e) (def_funs fl fl rho rho, e)
-  | Step_app: forall rho' fl f' vs xs e rho'' rho f t ys,
-                M.get f rho = Some (Vfun rho' fl f') ->
-                getlist ys rho = Some vs ->
-                find_def f' fl = Some (t,xs,e) ->
-                setlist xs vs (def_funs fl fl rho' rho') = Some rho'' ->
-                step (rho, Eapp f ys) (rho'', e)
-  | Step_prim: forall vs v rho' rho x t f f' ys e,
-                 getlist ys rho = Some vs ->
-                 M.get f pr = Some f' ->
-                 f' vs = Some v ->
-                 M.set x v rho = rho' ->
-                 step (rho, Eprim x t f ys e) (rho', e).
-
-  Definition stepf (s: env * exp) : option (env * exp) := 
-    let (rho,e) := s in
-    match e with
-      | Econstr x t n ys e => 
-        vs <- getlist ys rho ;; 
-        ret (M.set x (Vconstr t n vs) rho, e)
-      | Eproj x t n y e =>
-        match M.get y rho with
-          | Some (Vconstr t' n' vs) =>
-            v <- nthN vs n ;; ret (M.set x v rho, e)
-          | _ => None
-        end
-      | Ecase y cl =>
-        match M.get y rho with
-          | Some (Vconstr t c vl) =>
-            e' <- findtag cl c ;; ret (rho, e')
-          | _ => None
-        end
-      | Efun fl e => 
-        ret (def_funs fl fl rho rho, e)
-      | Eapp f ys =>
-        match M.get f rho with
-            | Some (Vfun rho' fl f') =>
-              vs <- getlist ys rho ;;
-                 match find_def f' fl with
-                   | Some (t',xs,e) =>
-                     rho'' <- setlist xs vs (def_funs fl fl rho' rho') ;;
-                     ret (rho'', e)
-                   | _ => None
-                 end
-            | _ => None
-        end
-      | Eprim x t f ys e =>
-        vs <- getlist ys rho ;;
-        f' <- M.get f pr ;;
-        v <- f' vs ;;
-        ret (M.set x v rho, e)
-    end.
-
-  Lemma step_stepf:
-    forall s s',
-      step s s' ->
-      stepf s = Some s'.
-  Proof.
-    intros [rho e] [rho' e'] H;
-    inv H; simpl;
-    repeat match goal with
-             | H: ?A= _ |- match ?A with _ => _ end = _ => rewrite H 
-           end; 
-    auto.
-  Qed.
-
-  Lemma stepf_step:
-    forall s s',
-      stepf s = Some s' ->
-      step s s'.
-  Proof.
-    intros [rho e] [rho' e'] H.
-    destruct e; simpl in H; 
-    repeat 
-      match goal with
-        | H: match ?A with _ => _ end = Some _ |- _ => destruct A eqn:?; inv H
-        | H: Some _ = Some _ |- _ => inv H
-      end;
-    try solve [econstructor; eauto].
-  Qed.
-
-  (* multi step *)
-  Inductive mstep: state -> state -> Prop :=
-  | s_step: forall s1 s2 s3, step s1 s2 -> mstep s2 s3 -> mstep s1 s3
-  | z_step: forall s, mstep s s.
-
-  Inductive observable_val: val -> Prop :=
-  | obv_int : forall i, observable_val (Vint i)
-  | obv_obvs : forall t, observable_val (Vobvs t).
-
-  (* may want to force all vals in the list to be observable? *)
-  Inductive obs_val: Type :=
-  | Obs : forall vs:list val, type -> Forall observable_val vs -> obs_val.
-  
-  (* big step *)
-  Inductive bstep_e : env -> exp -> obs_val -> Prop :=
-  | BStep_app_obs:
-      forall rho t ys vs f,
-      forall vsobs:Forall observable_val vs, 
-        M.get f rho = Some (Vobvs t) ->
-        getlist ys rho = Some vs ->
-        bstep_e rho (Eapp f ys) (Obs vs t vsobs)
-
-  | BStep_constr :
-      forall x t n ys e rho rho' vs v ,
-        getlist ys rho = Some vs ->
-        M.set x (Vconstr t n vs) rho = rho' ->
-        bstep_e rho' e v ->
-        bstep_e rho (Econstr x t n ys e) v
-  | BStep_proj: forall t' n' vs v rho x t n y e ov,
-                  M.get y rho = Some (Vconstr t' n' vs) ->
-                  nthN vs n = Some v ->
-                  bstep_e (M.set x v rho) e ov ->
-                  bstep_e rho (Eproj x t n y e) ov 
-                          
-  | BStep_case :
-      forall y v e' c cl vl t rho rho',
-        M.get y rho = Some (Vconstr t c vl) ->
-        findtag cl c = Some e' ->
-        bstep_e rho' e' v ->
-        bstep_e rho (Ecase y cl) v
-  | BStep_app_fun :
-      forall rho' fl f' vs xs e rho'' rho f t ys v,
-        M.get f rho = Some (Vfun rho' fl f') ->
-        getlist ys rho = Some vs ->
-        find_def f' fl = Some (t,xs,e) ->
-        setlist xs vs (def_funs fl fl rho' rho') = Some rho'' ->
-        bstep_e rho'' e v ->
-        bstep_e rho (Eapp f ys) v
-  | BStep_fun: forall rho fl e v,
-                 bstep_e (def_funs fl fl rho rho) e v ->
-                 bstep_e rho (Efun fl e) v
-  | BStep_prim: forall vs  rho' rho x t f f' ys e v v',
-                  getlist ys rho = Some vs ->
-                  M.get f pr = Some f' ->
-                  f' vs = Some v ->
-                  M.set x v rho = rho' ->
-                  bstep_e rho' e v'  ->
-                  bstep_e rho (Eprim x t f ys e) v'.
-
-
-  (* if only consider ints and observers (i.e observable_val), syntactic 
-     equality on val is the desired notion of equality. *)
-  Theorem forall2_eq_rel:
-    forall (X:Type) (R:relation X), Equivalence R -> Equivalence (Forall2 R).
-  Proof.
-    intros. inversion H. constructor.
-    + red. intros. induction x. constructor. constructor.
-      apply Equivalence_Reflexive. assumption.
-    + red. intro x. induction x; intros. inversion H0. constructor.
-      inversion H0; subst.   apply IHx in H5. constructor.
-      apply (Equivalence_Symmetric _ _ H3). assumption.
-    + red. induction x; intros.
-      * inversion H0; subst; inversion H1. constructor.
-      * inversion H0; subst; inversion H1; subst. constructor.
-        eapply Equivalence_Transitive. apply H4. assumption.
-        apply (IHx _ _ H6) in H8. assumption.
-  Qed.
-
-  Definition val_proper: val -> Prop := observable_val. 
-  Definition val_equiv: val -> val -> Prop := @eq val. 
-
-  Theorem val_equiv_eq_rel: Equivalence (val_equiv).
-  Proof.
-    constructor; red.
-    + intros. reflexivity.
-    + intros. inversion H. reflexivity.
-    + intros. inversion H. inversion H0. reflexivity.
-  Qed.  
-  
-  Definition obs_val_proper: obs_val -> Prop := fun _ => True.
-  Definition obs_val_equiv: relation obs_val :=
-    fun vso1 vso2 => match vso1, vso2 with
-                       | Obs vs1 t1 vsop1, Obs vs2 t2 vsop2 => Forall2 (val_equiv) vs1 vs2 end.
-
-
-  Theorem obs_val_equiv_eq_rel: Equivalence (obs_val_equiv).
-  Proof.
-    assert (Equivalence (Forall2 val_equiv)). apply forall2_eq_rel.
-    apply val_equiv_eq_rel. constructor; red; intros.
-    + unfold obs_val_equiv. destruct x. apply H.
-    + unfold obs_val_equiv. unfold obs_val_equiv in H0.
-      destruct x; destruct y. revert H0. apply H.
-    + unfold obs_val_equiv. unfold obs_val_equiv in H0.
-      unfold obs_val_equiv in H1.
-      destruct x; destruct y; destruct z. revert H1; revert H0. apply H.
-  Qed.
-
-
-  Definition type_obs_val : T.type (obs_val) :=
-    {| T.equal := obs_val_equiv ;
-       T.proper := obs_val_proper |}.
-
-  Instance typeOk_obs_val: T.typeOk (type_obs_val).
-  Proof.
-    constructor.
-    + intros. split; do 3 red; constructor.
-    + do 3 red. intros. red.  destruct x. apply forall2_eq_rel.
-      apply val_equiv_eq_rel.
-    + do 3 red. intros. red in H. red in H. revert H.
-      apply obs_val_equiv_eq_rel.
-    + do 3 red. intros. do 2 (red in H). do 2 (red in H0).
-      revert H0; revert H; apply obs_val_equiv_eq_rel.
-  Qed.
-  
-(** 
-(* syntactic equivalence up to alpha-renaming*)
-Actually: only define val_equiv over observable_val, make functions non observable.
-
-Function renamed (R:list (var * var)) (v v':var) : Prop :=
-  match R with
-    | (x, x')::R' =>
-      (@eq var x v <-> @eq var x' v') /\ ((@eq var x v = False /\ @eq var x' v' = False) -> renamed R' v v') 
-    | nil => False
-  end.
-
-Function renamed_list (R:list (var * var)) (vs vs': list var): Prop :=
-  match (vs, vs') with
-    | (v:: vss, v'::vss') => renamed R v v' /\ renamed_list R vss vss'
-    | (nil, nil) => True
-    | _ => False
-  end.
-
-  
-Function exp_alphasyneq (R:list (var * var)) (e1 e2:exp) : Prop :=
-  match (e1, e2) with
-    | (Econstr v t tg vs e, Econstr v' t' tg' vs' e') =>
-      renamed_list R vs vs' /\
-      exp_alphasyneq ((v, v')::R) e e' 
-    | (Eproj x t n y e, Eproj x' t' n' y' e') =>
-      renamed R y y' /\ exp_alphasyneq ((x,x')::R) e e'
-    | (Ecase y cl, Ecase y' cl') =>
-      renamed R y y' /\ Forall2 (fun tl tl':(tag * var)=> match (tl, tl') with
-                                                            | ((_, y), (_, y')) => renamed R y y' end ) cl cl'
-    | (Efun fl e, Efun fl' e') =>
-            exp_alphasyneq R e e'
-    | (Eapp f ys, Eapp f' ys') =>
-       renamed R f f' /\ renamed_list R ys ys'
-    | (Eprim x t (f::ys) e, Eprim x' t' (f'::ys') e') =>
-      exp_alphasyneq R e e'
-    | _ => False
-  end.
-
-Function fundefs_alphasyneq (R:list (var * var)) (f1 f2:fundefs) : Prop :=
-  match (f1, f2) with
-    | (Fcons f t xs e f1', Fcons f' t' xs' e' f2' ) =>
-      if beq_nat (length xs) (length xs') then
-        False
-      else
-      (exp_alphasyneq ((combine xs xs')++R) e e') /\ (fundefs_alphasyneq R f1' f2')
-    | (Fnil, Fnil) => True
-    | _ => False
-  end.
-
-Function add_fundefseq (R:list (var * var))  (defs defs':fundefs) : option (list (var * var)) :=
-  match (defs, defs') with
-    | (Fcons f t ys e fdefs, Fcons f' t' ys' e' fdefs') =>
-      add_fundefseq ((f,f')::R) fdefs fdefs'
-    | (Fnil , Fnil) => Some R
-    | _ => None
-  end.
-
-Function val_equiv' (v1 v2:val) {struct v1}: Prop :=
-    match (v1, v2) with
-      | (Vfun valsubst defs f, Vfun valsubst' defs' f') =>
-        match (add_fundefseq nil defs defs') with
-          | Some R' =>  fundefs_alphasyneq  R' defs defs' (* may instead start by checking f f' and recursively check for equality on function calls within f and f' *)
-          | None => False (* lists are of different size, could instead explore from f and f', o.w. can't reorder/delete functions *)
-        end
-
-      |  _  => @eq val v1 v2
-    end.
-
-Instance eq_val: Equivalence val_equiv.
-
-val_equiv is wrong, only superficial function, not rec.
- *)
-    
-  
-  Definition var_equiv: env -> env -> relation var :=
-    fun rho1 rho2 =>
-      fun var1 var2 =>
-        match (M.get var1 rho1, M.get var2 rho2) with
-          |(Some v1, Some v2) => val_equiv v1 v2
-          | _ => False
-        end.
-
-
-  (* small-step based equality on state *)    
-  Definition valid_term_state (s:state) :=
-    match s with
-      | (rho, Eapp g varl) =>
-        match M.get g rho with
-          | Some (Vobvs t) =>
-            Forall (fun var => match M.get var rho with
-                                 | Some val => observable_val val
-                                 | _ => False
-                               end) varl
-          | _ => False
-        end
-      | _ => False
-    end.
-
-
-
-  Definition state_equiv: relation state :=
-    fun s1 s2 =>
-      exists sv1 sv2,
-        mstep s1 sv1 /\ mstep s2 sv2 /\
-        valid_term_state sv2 /\ valid_term_state sv1 /\
-        match (sv1, sv2) with
-          | ((rho1, Eapp g1 varl1) , (rho2, Eapp g2 varl2)) =>
-            match (M.get g1 rho1, M.get g2 rho2) with 
-               | (Some v1, Some v2) => val_equiv v1 v2
-               | _ => False
-             end
-            /\ Forall2 (var_equiv rho1 rho2) varl1 varl2
-          | _ => False
-        end.
-  
-
-
-  (* Theorems about  (small-)step relation *)
-
-  
-  (* Definition env_of_tenv :=  *)
-  (*   fun rho:env => *)
-  (*     fun Gamma:tenv => *)
-  (*       forall var, *)
-  (*         (exists ty, M.get var Gamma = Some ty <-> *)
-  (*                     exists val, M.get var rho = Some val /\ type_of_val val ty). *)
-
-  Theorem step_deterministic: forall s s' s'',
-                                step s s' -> step s s'' -> s' = s''.
-  Proof.
-    intros.
-    inversion H; inversion H0; subst;
-    repeat match goal with
-             | [ |- ?P = ?P] => reflexivity
-             | [H: ( Some _ = Some _ ) |- _ ] => inversion H; subst      
-             | [H1: (?P = Some _), H2:(?P = Some _) |- _ ] => rewrite H1 in H2;
-                 inversion H2; subst
-             | [H: ((?rho0, _) = (?rho, _)) |- _ ] => inversion H; subst
-           end.
-    + rewrite H6 in H2.  inversion H2; subst. reflexivity.
-    + rewrite H6 in H2; inversion H2; subst. reflexivity.
-    + rewrite H9 in H3; inversion H3; subst.
-      rewrite H2 in H8; inversion H8; subst.
-      rewrite H10 in H4; inversion H4. reflexivity.
-    + rewrite H2 in H8; inversion H8; subst.
-      rewrite H9 in H3; inversion H3; subst; reflexivity.
-  Qed.  
-
-  Theorem cant_step_terminal:
-    forall s s',
-      valid_term_state s -> 
-      ~ step s s'.
-  Proof.
-    intros s s' H Hstep. unfold valid_term_state in H.
-    destruct s. destruct e0; try inversion H. 
-    destruct (M.get v e) eqn:Heq; try inversion H. destruct v0; try inv H; 
-    inv Hstep; congruence. 
-  Qed.
-
-  Theorem state_equiv_step_l:
-    forall s1 s2 s1', step s1 s1' -> (state_equiv s1 s2 <-> state_equiv s1' s2).
-  Proof.
-    intros s1 s2 s1' H0. split; intro.
-    + unfold state_equiv in H. destruct H as [sv1 ?]. destruct H as [sv2 ?].
-      do 4 ( destruct H as [?V H]). inversion V; subst.  assert (s3 = s1').
-      eapply step_deterministic. apply H1. apply H0. subst. unfold state_equiv.
-      exists sv1. exists sv2. split. assumption. split. assumption. split.
-      assumption. split. assumption. assumption.
-      apply (cant_step_terminal _ _ V2) in H0. inversion H0.
-    + unfold state_equiv in H. destruct H as [sv1 ?]. destruct H as [sv2 ?].
-      do 4 (destruct H as [?V H]). assert (mstep s1 sv1). eapply s_step.
-      apply H0. apply V. unfold state_equiv. exists sv1. exists sv2. split.
-      assumption. split. assumption. split. assumption. split. assumption.
-      assumption.
-  Qed.
-
-  Theorem state_equiv_step_r:
-    forall s1 s2 s2', step s2 s2' ->
-                      (state_equiv s1 s2  <-> state_equiv s1 s2').
-  Proof.
-    intros s1 s2 s2' H0. split; intro.
-    + unfold state_equiv in H. destruct H as [sv1 ?]. destruct H as [sv2 ?].
-      do 4 (destruct H as [?V H]). inversion V0; subst. assert (s3 = s2').
-      eapply step_deterministic. apply H1. assumption. subst.
-      unfold state_equiv. exists sv1. exists sv2. split. assumption.
-      split. assumption. split. assumption. split. assumption. assumption.
-      apply (cant_step_terminal _ _ V1) in H0. inversion H0.
-    + unfold state_equiv in H. destruct H as [sv1 ?]. destruct H as [sv2 ?].
-      do 4 (destruct H as [?V H]). assert (mstep  s2 sv2). eapply s_step; eauto.
-      unfold state_equiv. exists sv1. exists sv2. split. assumption. split.
-      assumption. split. assumption. split. assumption. assumption.
-  Qed.
-  
-
-  (* 
-Theorem progress: forall TD Gamma e rho,
-                    welltyped TD Gamma e -> env_of_tenv rho Gamma -> valid_term_state (rho, e) \/  (exists rho' e', step (rho, e) (rho', e')).
-admit.
-Qed.
- 
-Theorem preservation: forall TD Gamma Gamma' rho rho' e e',
-   welltyped TD Gamma e -> env_of_tenv rho Gamma -> step (rho, e) (rho', e') -> env_of_tenv rho' Gamma' -> welltyped TD Gamma' e'.
-admit.
-Qed.
-   *)
-
-
-
-  (* theorems about mstep *)
-
-  (* can't prove this, can assume it for terms I receive *)
-  (* Theorem termination: forall TD Gamma e rho,
-     welltyped TD Gamma e -> env_of_tenv rho Gamma -> (exists rho' ev, mstep (rho,e) (rho', ev) /\ valid_term_state (rho', ev)).
-admit.
-Qed. *)
-
-  Theorem church_rosser:
-    forall s sv1 sv2,
-      mstep s sv1 ->
-      mstep s sv2 ->
-      (exists s', mstep sv1 s' /\ mstep sv2 s').
-  Proof.
-    intro s. intros. generalize dependent sv2. induction H.
-    - intros. destruct H1.
-      + assert (s2 = s0). eapply step_deterministic. apply H. apply H1.
-        subst. apply IHmstep in H2.  destruct H2. exists x. assumption.
-      + assert ( exists s' : state, mstep s3 s' /\ mstep s3 s').
-        apply (IHmstep _ H0). destruct H1. destruct H1. exists s3.
-        split. constructor. eapply s_step. apply H. apply H0.
-    - intros. exists sv2. split. assumption. constructor.
-  Qed.
-
-
-  Theorem mstep_terminal_to_itself:
-    forall s s',
-      valid_term_state s -> 
-      mstep s s' ->
-      s = s'.
-  Proof.
-    intros. inversion H0; subst.
-    assert False. eapply cant_step_terminal. apply H. apply H1. inversion H3.
-    reflexivity.
-  Qed.
-
-
-  
-  Theorem forall2_varequiv_transitive:
-    forall e1 e2 e3 l1 l2 l3,
-      Forall2 (var_equiv e1 e2) l1 l2 ->
-      Forall2 (var_equiv e2 e3) l2 l3 ->
-      Forall2 (var_equiv e1 e3) l1 l3.
-  Proof.
-    intros. generalize dependent l2. generalize dependent l3.
-    induction l1; intros.
-    inversion H; subst. inversion H0; subst. constructor.
-    inversion H; subst. inversion H0; subst. constructor.
-    red. red in H3. red in H4. clear H0. clear H7. clear H.
-    clear IHl1. destruct (M.get a e1); try inversion H3.
-    destruct (M.get y e2); try inversion H3. destruct (M.get y0 e3);
-      try inversion H4. reflexivity.
-    eapply IHl1. apply H5. apply H7.
-  Qed.
-
-
-  Definition state_proper :=
-    fun st => exists sv, mstep st sv /\ valid_term_state sv.
-
-  (* small step state equivalence *)
-  Definition type_state : T.type (state) :=
-    {| T.equal := state_equiv
-       ; T.proper := state_proper
-    |}.
-
-  Instance typeOk_state : T.typeOk (type_state). 
-  constructor.  
-  intros.
-
-  (* only proper *)
-  inversion H. destruct H0. destruct H0. destruct H1.
-  destruct H2. destruct H3. split; do 2 red. exists x0; split; assumption.
-  exists x1; split; assumption.
-
-  (* Reflective for proper state *)         
-  red. intros. inversion H. destruct H0. red. red. red. exists x0.
-  exists x0. split. assumption. split. assumption. split. assumption.
-  split. assumption. unfold valid_term_state in H1. destruct x0.
-  destruct e0; try inversion H1. destruct (M.get v e); try inversion H1.
-  split. red. reflexivity. clear H0. induction l. constructor. constructor.
-  red. destruct v0; try inversion H1; subst.  destruct (M.get a e). reflexivity.
-  inversion H3. apply (IHl). destruct v0; try inversion H1. inversion H1; subst.
-  assumption.
-
-  (* symmetric *)
-  red. intros. red. red. red. destruct H. destruct H. destruct H. destruct H0.
-  destruct H1. destruct H2. exists x1. exists x0. split. assumption. split.
-  assumption. split. assumption. split. assumption. destruct x0. destruct x1.
-  destruct e0; try inversion H3. destruct e2; try inversion H3. split. clear H.
-  clear H0. destruct (M.get v e); try inversion H3.
-  destruct (M.get v0 e1); try inversion H4. reflexivity. inversion H. clear H.
-  clear H0. clear H1. clear H2. clear H3. generalize dependent l0. induction l.
-  intros. inversion H5. subst. constructor. intros. inversion H5. constructor.
-  (* var_equiv is quasi-symmetric*) unfold var_equiv. unfold var_equiv in H1.
-  destruct (M.get a e); try inversion H1.
-  destruct (M.get y0 e1); try inversion H1. reflexivity.  apply IHl. assumption.
-
-  (* Transitive *)
-  red. intros. do 3 red. do 3 red in H.  do 3 red in H0. destruct H. destruct H.
-  destruct H0. destruct H0. destruct H. destruct H1. destruct H2. destruct H3.
-  destruct H0. destruct H5. destruct H6. destruct H7.
-  assert (exists s', mstep x1 s' /\ mstep x2 s').
-  apply (church_rosser y x1 x2 H1 H0).
-  destruct H9. destruct H9.
-  apply (mstep_terminal_to_itself _ _ H7) in H10; subst.
-  apply (mstep_terminal_to_itself _ _ H2) in H9; subst. exists x0. exists x3.
-  repeat (split; try assumption).
-  destruct x0. destruct e0; try inversion H4. destruct x3. destruct x4.
-  destruct e3; try inversion H4. destruct e1; try inversion H8.
-  destruct (M.get v e); try inversion H9. split. destruct (M.get v0 e2); try inversion H8.
-  destruct (M.get v1 e0); try inversion H11. eapply transitivity. apply H9.
-  apply H11. inversion H11. eapply forall2_varequiv_transitive. destruct H4.
-  apply f. apply H12. 
-  Qed.
-  (* proofs of semantics preservation for P will look like 
-   forall rho, proper (rho, e) -> equal (rho, e) (rho, P e). *)
-  
-
-  (* small step exp equivalence *)
-  Definition exp_equiv: relation exp :=
-    fun e1 e2 =>
-      (forall rho1,
-         state_proper(rho1, e1) -> state_equiv (rho1, e1) (rho1, e2)) /\
-      (forall rho2,
-         state_proper (rho2, e2) -> state_equiv (rho2, e1) (rho2, e2)).
-
-  Definition exp_proper := fun e:exp => True.
-
-  Definition type_exp : T.type (exp) :=
-    {| T.equal := exp_equiv 
-       ; T.proper := exp_proper
-    |}.
-
-  Ltac tci := eauto with typeclass_instances.
-
-  Instance typeOk_exp : T.typeOk (type_exp).
-  Proof.
-    constructor.
-    intros. split; do 3 red; constructor.
-    (* PRefl *)
-    + red. intros. do 3 red. split; intros; apply typeOk_state; tci.
-
-    (* Symmetric *)    
-    + red. intros. do 3 red in H. destruct H. do 3 red. split; intros.
-    - apply H0 in H1. generalize H1. apply typeOk_state; tci.
-    - apply H in H1. generalize H1. apply typeOk_state; tci.
-      (* Transitive *)
-      + do 3 red. intros. do 3 red in H. destruct H. do 3 red in H0.
-        destruct H0. red. split; intros.
-    - apply H in H3. assert (H4 := H3). apply typeOk_state in H3. destruct H3.
-      apply H0 in H5. generalize H5. generalize H4. apply typeOk_state; tci.
-    - apply H2 in H3. assert (H4 := H3). apply typeOk_state in H3; destruct H3.
-      apply H1 in H3. generalize H4. generalize H3. apply typeOk_state; tci.
-  Qed.
-
-  (* fun equivalence *)
-  Definition fun_equiv: forall e1 e2, exp_equiv e1 e2 -> relation fundefs :=
-    fun e1 e2 =>
-      fun equiv_e1e2 =>
-        fun fds1 fds2 =>
-          (forall rho1,
-             state_proper (def_funs fds1 fds1 rho1 rho1, e1) ->
-             state_equiv (def_funs fds1 fds1 rho1 rho1, e1) (def_funs fds2 fds2 rho1 rho1, e2)) /\
-          (forall rho2,
-             state_proper (def_funs fds2 fds2 rho2 rho2, e2) ->
-             state_equiv (def_funs fds1 fds1 rho2 rho2, e1) (def_funs fds2 fds2 rho2 rho2, e2)).
-
-  Definition fun_proper := fun f:fundefs => True.
-
-  Definition etype_fun :  forall e1 e2, exp_equiv e1 e2 -> T.type fundefs  :=
-    fun e1 e2 => fun equiv_e1e2 => 
-                   {| T.equal := fun_equiv e1 e2 equiv_e1e2
-                      ; T.proper := fun_proper
-                   |}.
-
-  Instance etypeOk_fun : forall e1 e2, forall equiv_e1e2: exp_equiv e1 e2, T.typeOk (etype_fun e1 e2 equiv_e1e2).
-  intros. constructor.
-  (* only *)
-  + intros. split; do 3 red; constructor.
-  (* Prefl *)
-  + red. intros. do 3 red. split; intros.
-  - red in equiv_e1e2. destruct equiv_e1e2.
-    apply s in H0. assumption.  
-  - red in equiv_e1e2. destruct equiv_e1e2. apply s0 in H0. assumption. 
-    (* symmetric *)
-    + red. intros. do 3 red in H. do 3 red. destruct H. red in equiv_e1e2.
-      destruct equiv_e1e2. split; intros.
-  - assert (H4 := H3). apply H1 in H4.  assert (H5 := H4).
-    apply typeOk_state in H4; destruct H4.  apply H0 in H6.
-    assert (H7 := H6). apply typeOk_state in H6; destruct H6. apply H1 in H6.
-    eapply (@T.equiv_trans _ type_state typeOk_state).
-    eapply (@T.equiv_trans _ type_state typeOk_state).
-    apply H5. apply (T.equiv_sym type_state _ _) in H7. apply H7. assumption.
-  - apply H2 in H3. assert (H4 := H3). apply typeOk_state in H4; destruct H4.
-    apply H in H4. assert (H6 := H4). apply typeOk_state in H4; destruct H4.
-    apply H2 in H7. eapply (@T.equiv_trans _ type_state typeOk_state).
-    eapply (@T.equiv_trans _ type_state typeOk_state). apply H7.
-    apply (T.equiv_sym type_state _ _) in H6. apply H6. assumption.    
-    (* transitive *)
-    + red. intros. do 3 red in H. do 3 red in H0. do 3 red.
-      destruct H. destruct H0. red in equiv_e1e2. destruct equiv_e1e2.
-      split; intros.
-  - apply H in H5. assert (Hfin1 := H5). apply typeOk_state in H5; destruct H5.
-    apply H4 in H6. assert (Hfin2 := H6). apply typeOk_state in H6; destruct H6.
-    apply H0 in H6. Print T. About T.equiv_sym.
-    eapply (T.equiv_sym type_state _ _) in Hfin2. About T.equiv_trans.
-    eapply (@T.equiv_trans _ type_state typeOk_state).
-    eapply (@T.equiv_trans _ type_state typeOk_state). apply Hfin1.
-    apply Hfin2. apply H6.
-  - apply H2 in H5. assert (Hfin1 := H5). apply typeOk_state in H5; destruct H5.
-    apply H3 in H5. assert (Hfin2 := H5). apply typeOk_state in H5; destruct H5.
-    apply H1 in H7.  eapply (@T.equiv_trans _ type_state typeOk_state).
-    eapply (@T.equiv_trans _ type_state typeOk_state). apply H7.
-    apply (T.equiv_sym type_state _ _) in Hfin2. apply Hfin2. assumption.
-  Qed.
-  
-  (* big step exp equivalence *)
-  Definition  bs_exp_proper :=
-    fun _:exp => True (* fun e:exp => exists rho v, bstep_e rho e v. *).
-
-
-
-  Definition bs_exp_equiv : relation exp :=
-    fun e1 e2 =>
-      (forall rho v,
-         bstep_e rho e1 v -> exists v', bstep_e rho e2 v' /\ obs_val_equiv v v') /\
-      (forall rho v,
-         bstep_e rho e2 v -> exists v', bstep_e rho e1 v' /\ obs_val_equiv v v').
-
-  Definition type_bs_exp : T.type (exp) :=
-    {| T.equal := bs_exp_equiv
-       ;T.proper := bs_exp_proper |}.
-
-  Instance typeOk_bs_exp : T.typeOk (type_bs_exp).
-  Proof.
-    constructor.
-    intros. split; do 3 red; constructor.
-    + do 3 red. intros. unfold bs_exp_equiv.
-      split; intros. exists v. split. assumption.
-      apply obs_val_equiv_eq_rel. exists v. split. assumption.
-      apply typeOk_obs_val. auto.
-    + red. intros. do 3 red in H.  destruct H. do 3 red. split; intros.
-      apply H0 in H1. destruct H1. destruct H1. exists x0. split. assumption.
-      assumption. apply H in H1. destruct H1. destruct H1.
-      exists x0. split; assumption.
-    + do 3 red. intros. do 3 red in H. destruct H. do 3 red in H0.
-      destruct H0. red. split. intros. apply H in H3. destruct H3. destruct H3.
-      apply H0 in H3. destruct H3. exists x1. destruct H3. split. assumption.
-      revert H5. revert H4. apply typeOk_obs_val.
-      intros. apply H2 in H3. destruct H3. destruct H3. apply H1 in H3.
-      destruct H3. exists x1. destruct H3. split. assumption. revert H5.
-      revert H4. apply typeOk_obs_val.
-  Qed.
-  
-End PRIMS.
