theories/L6_PCPS/ctx_approx.v
@@ -1,75 +1,82 @@
 Require Import Coq.Arith.Arith Coq.NArith.BinNat Coq.Lists.List Coq.omega.Omega
         Coq.Relations.Relations Coq.Classes.RelationClasses.
-Require Import cps ctx eval identifiers.
+Require Import cps ctx eval logical_relations identifiers.
 Import ListNotations.
+
 
 Definition empty_env := M.empty val.
 
-Open Scope ctx_scope. 
+Ltac inv H := inversion H; clear H; subst.
 
-(** Contextual approximation *)
-Definition ctx_approx : relation exp :=
-  fun e1 e2 =>
-    forall C i v1, eval.bstep_e empty_env (C |[ e1 ]|) v1 i ->
-              exists v2 j, eval.bstep_e empty_env (C |[ e2 ]|) v2 j.
+Section ctx_approx.
 
-(** Contextual equivalence *)
-Definition ctx_equiv : relation exp :=
-  fun e1 e2 => ctx_approx e1 e2 /\ ctx_approx e2 e1.
+  Variable pr : prims.
 
-Lemma ctx_approx_trans :
+  Open Scope ctx_scope.
+  
+  (** Contextual approximation *)
+  Definition ctx_approx : relation exp :=
+    fun e1 e2 =>
+      forall C i v1, bstep_e pr empty_env (C |[ e1 ]|) v1 i ->
+                exists v2 j, bstep_e pr empty_env (C |[ e2 ]|) v2 j.
+  
+  (** Contextual equivalence *)
+  Definition ctx_equiv : relation exp :=
+    fun e1 e2 => ctx_approx e1 e2 /\ ctx_approx e2 e1.
+  
+  Lemma ctx_approx_trans :
   Transitive ctx_approx.
-Proof. 
-  intros x y z H1 H2 C i v1 Hstep.
-  edestruct H1 as [v2 [j2 Hstep2]]; eauto. 
-Qed.
+  Proof. 
+    intros x y z H1 H2 C i v1 Hstep.
+    edestruct H1 as [v2 [j2 Hstep2]]; eauto. 
+  Qed.
 
-Lemma ctx_approx_refl :
-  Reflexive ctx_approx.
-Proof. 
-  intros x C i v1 Hstep.
-  repeat split; eauto.
-Qed.
+  Lemma ctx_approx_refl :
+    Reflexive ctx_approx.
+  Proof. 
+    intros x C i v1 Hstep.
+    repeat split; eauto.
+  Qed.
+  
+  Lemma ctx_equiv_equiv :
+    Equivalence ctx_equiv.
+  Proof.
+    constructor.
+    - split; apply ctx_approx_refl; eauto.
+    - split; eapply H.
+    - intros x y z [H1 H2] [H3 H4]; split; eapply ctx_approx_trans; eauto.
+  Qed.
 
-Lemma ctx_equiv_equiv :
-  Equivalence ctx_equiv.
-Proof.
-  constructor.
-  - split; apply ctx_approx_refl; eauto.
-  - split; eapply H.
-  - intros x y z [H1 H2] [H3 H4]; split; eapply ctx_approx_trans; eauto.
-Qed.
-
-Lemma preord_exp_sound e1 e2 :
-  (forall k rho1 rho2, preord_env_P (occurs_free e1) k rho1 rho2 ->
-                  preord_exp k (e1, rho1) (e2, rho2)) ->
-  ctx_approx e1 e2.
-Proof.
-  intros Hyp C i v1 Hstep.
-  assert (Hyp' := Hyp).
-  eapply (preord_exp_compat i empty_env empty_env C) in Hyp;
-  [| now eapply preord_env_P_refl ].
-  edestruct Hyp as [v2 [c2 [Hstep2 Hpre2]]]; eauto.
-Qed.
-
-Definition x : var := 1%positive.
-Definition y : var := 2%positive.
-
-Definition tau : type := 1%positive.
-Definition c : tag := 1%positive.
-
-Definition stuck : exp :=
-  Econstr x tau c [] (
-  Econstr y tau c [] (
-  Eapp x [y])).
-
-Lemma stuck_gets_stuck rho :
-  ~ (exists v c, bstep_e rho stuck v c).
-Proof.
-  intros [v [c H]]. inv H. inv H8.
-  inv H10. inv H7. inv H9.
-  - rewrite M.gso, M.gss in H2. inv H2.
+  Lemma preord_exp_sound e1 e2 :
+    (forall k rho1 rho2, preord_env_P pr (occurs_free e1) k rho1 rho2 ->
+                    preord_exp pr k (e1, rho1) (e2, rho2)) ->
+    ctx_approx e1 e2.
+  Proof.
+    intros Hyp C i v1 Hstep.
+    assert (Hyp' := Hyp).
+    eapply (preord_exp_compat pr i empty_env empty_env C) in Hyp;
+      [| now eapply preord_env_P_refl ].
+    edestruct Hyp as [v2 [c2 [Hstep2 Hpre2]]]; eauto.
+  Qed.
+  
+  Definition x : var := 1%positive.
+  Definition y : var := 2%positive.
+  
+  Definition tau : type := 1%positive.
+  Definition c : tag := 1%positive.
+  
+  Definition stuck : exp :=
+    Econstr x tau c [] (
+              Econstr y tau c [] (
+                        Eapp x [y])).
+  
+  Lemma stuck_gets_stuck rho :
+    ~ (exists v c, bstep_e pr rho stuck v c).
+  Proof.
+    intros [v [c H]]. inv H. inv H8.
+    inv H10. inv H7. inv H9.
+    rewrite M.gso, M.gss in H1. inv H1.
     intros Hc. inv Hc.
-  - rewrite M.gso, M.gss in H1. inv H1.
-    intros Hc. inv Hc.
-Qed.
+  Qed.
+  
+End ctx_approx.
