theories/L6_PCPS/alpha_conv.v
@@ -235,277 +235,283 @@ Proof.
   rewrite <- Hfeq. rewrite <- Hfeq in H2. now eauto.
   rewrite Hfeq. rewrite Hfeq in H2. now eauto. 
 Qed.
+
+Section Alpha_conv_correct.
+
+  Variable pr : prims.
+
+  Definition preord_env_P_inj P k f rho1 rho2 :=
+    forall x : var,
+      P x -> preord_var_env pr k rho1 rho2 x (f x).
+
+  Lemma Forall2_app {A B} (P : A -> B -> Prop) xs ys f :
+    Forall2 (fun x y => f x = y) xs ys ->
+    (forall x y, List.In x xs -> f x = y -> P x y) ->
+    Forall2 P xs ys. 
+  Proof. 
+    intros Hall Hyp. induction Hall.
+    - constructor.
+    - constructor.
+      + eapply Hyp. now constructor. eassumption.
+      + eapply IHHall.
+        intros. eapply Hyp. now constructor 2.
+        eassumption. 
+  Qed.
+
+  Lemma construct_fundefs_injection_injective f B1 B2 f' :
+    construct_fundefs_injection f B1 B2 f' ->
+    injective f ->
+    injective f'. 
+  Proof.
+    intros H1 H2. induction H1; eauto. 
+  Qed.
+
+  Lemma construct_lst_injection_injective f xs ys f' :
+    construct_lst_injection f xs ys f' ->
+    injective f ->
+    injective f'. 
+  Proof.
+    intros H1 H2. induction H1; eauto. 
+  Qed.
+
+  Lemma preord_env_P_inj_set (P : Ensemble var) (rho1 rho2 : env) 
+        (k : nat)  f(x y : var) (v1 v2 : val) : 
+    preord_env_P_inj (Setminus var P (Singleton var x)) k f rho1 rho2 ->
+    preord_val pr k v1 v2 ->
+    injective (f {x ~> y}) ->
+    preord_env_P_inj P k (f {x ~> y}) (M.set x v1 rho1) (M.set y v2 rho2).
+  Proof. 
+    intros Henv Hv Hinj z HP. unfold extend. 
+    destruct (Coqlib.peq z x) as [| Hneq] eqn:Heq'.
+    - subst. intros z Hget.
+      rewrite M.gss in Hget. inv Hget. eexists. rewrite M.gss; eauto.
+    - intros z' Hget. rewrite M.gso in Hget; eauto.
+      destruct (Coqlib.peq (f z) y).
+      + exfalso. eapply Hneq. eapply Hinj. now constructor.
+        now constructor. rewrite extend_gso; eauto.
+        rewrite extend_gss. eassumption.
+      + edestruct (Henv z); eauto.
+        constructor; eauto. intros Hc. inv Hc. congruence. 
+        eexists. rewrite M.gso; eauto. 
+  Qed.
+
+  Lemma preord_env_P_inj_antimon (P1 P2 : var -> Prop) (k : nat) (rho1 rho2 : env) f :
+    preord_env_P_inj P2 k f rho1 rho2 ->
+    Included var P1 P2 -> preord_env_P_inj P1 k f rho1 rho2.
+  Proof.
+    intros Henv Hi x HP. eapply Henv. now apply Hi.
+  Qed.
+
+  Lemma preord_env_P_inj_monotonic :
+    forall P (k j : nat) (rho1 rho2 : env) f,
+      j <= k -> preord_env_P_inj P k f rho1 rho2 -> preord_env_P_inj P j f rho1 rho2.
+  Proof.
+    intros P k j rho1 rho2 f Hleq Hpre x HP v Hget.
+    edestruct Hpre as [v2 [Heq Hpre2] ]; eauto.
+    eexists; split; eauto. eapply preord_val_monotonic; eauto.
+  Qed.
+
+  Instance preord_env_P_inj_proper  :
+    Proper (Same_set var ==> Logic.eq ==> Logic.eq ==> Logic.eq ==> Logic.eq ==> iff)
+           preord_env_P_inj.
+  Proof.
+    intros s1 s2 [H1 H2]; split; intros Hpre;
+    eapply preord_env_P_inj_antimon; subst; eauto.
+  Qed.
+
+  Lemma Alpha_conv_fundefs_find_def B1 B2 f g t xs1 e1 :
+    Alpha_conv_fundefs B1 B2 f ->
+    find_def g B1 = Some (t, xs1, e1) ->
+    injective f ->
+    exists xs2 e2 f', 
+      find_def (f g) B2 = Some (t, xs2, e2) /\
+      length xs1 = length xs2 /\
+      construct_lst_injection f xs1 xs2 f' /\
+      Alpha_conv e1 e2 f'.
+  Proof. 
+    intros Ha Hdef Hinj. induction Ha. 
+    - inv Hdef. 
+    - simpl in Hdef. subst. destruct (M.elt_eq g g0).
+      + subst. inv Hdef. exists xs', e'.
+        simpl. rewrite Coqlib.peq_true. eauto.
+      + edestruct IHHa as [xs2 [ e2 Ha' ] ]; eauto.
+        edestruct (Coqlib.peq (f g) (f g0)). 
+        * eapply Hinj in e0. subst. congruence. now constructor.
+          now constructor.
+        * do 2 eexists. simpl. rewrite Coqlib.peq_false; eauto.
+  Qed.
+
+  Lemma setlist_length2 (rho rho' rho1 : env) (xs1 xs2 : list var) (vs1 vs2 : list val) :
+    length xs1 = length xs2 ->
+    length vs1 = length vs2 ->
+    setlist xs1 vs1 rho = Some rho1 ->
+    exists rho2 : M.t val, setlist xs2 vs2 rho' = Some rho2.
+  Proof. 
+    revert xs2 vs1 vs2 rho1.
+    induction xs1 as [| x xs1 IHxs ]; intros xs2 vs1 vs2 rho1 Hlen1 Hlen2 Hset.
+    - inv Hset. destruct vs1; try discriminate. inv H0.
+      destruct vs2; try discriminate. destruct xs2; try discriminate.
+      eexists; simpl; eauto.
+    - destruct xs2; try discriminate.
+      destruct vs1; try discriminate. destruct vs2; try discriminate.
+      inv Hlen1. inv Hlen2. simpl in Hset. 
+      destruct (setlist xs1 vs1 rho) eqn:Heq2; try discriminate. inv Hset.
+      edestruct IHxs as [vs2' Hset2]; try eassumption.
+      eexists. simpl; rewrite Hset2; eauto.
+  Qed.
+
+  Lemma preord_env_P_inj_setlist (P1 : var -> Prop) (rho1 rho2 rho1' rho2' : env)
+        (k : nat) (xs1 xs2 : list var) (vs1 vs2 : list val) f f':
+    preord_env_P_inj P1 k f rho1 rho2 ->
+    Forall2 (preord_val pr k) vs1 vs2 ->
+    construct_lst_injection f xs1 xs2 f' ->
+    setlist xs1 vs1 rho1 = Some rho1' ->
+    setlist xs2 vs2 rho2 = Some rho2' ->
+    preord_env_P_inj (Union _ P1 (FromList xs1)) k f' rho1' rho2'.
+  Proof.
+    revert P1 rho1 rho2 rho1' rho2' xs2 vs1 vs2 f f'. induction xs1;
+      intros P1 rho1 rho2 rho1' rho2' xs2 vs1 vs2  f f' Hpre Hall Hinj Hset1 Hset2 x HP v Hget.
+    - inv Hinj. destruct vs1; try discriminate.
+      inv Hall. 
+      inv Hset1; inv Hset2. eapply Hpre; eauto.
+      inv HP; [ now eauto | now inv H ]. 
+    - destruct vs1; try discriminate. inv Hall. inv Hinj.
+      simpl in Hset1, Hset2. 
+      destruct (setlist xs1 vs1 rho1) eqn:Heq1;
+        destruct (setlist ys l' rho2) eqn:Heq2; try discriminate.
+      inv Hset1; inv Hset2. rewrite M.gsspec in Hget.
+      destruct (Coqlib.peq x a); subst.
+      + inv Hget. eexists. 
+        simpl. unfold extend. rewrite Coqlib.peq_true.
+        rewrite M.gss. eauto.
+      + edestruct IHxs1 as [v2 [Het' Hpre'] ]; eauto.
+        * inv HP; [ now left; eauto |].
+          rewrite FromList_cons in H. inv H.
+          inv H0. congruence. right; eauto.
+        * eexists. unfold extend. rewrite Coqlib.peq_false; [| now eauto ].
+          rewrite M.gso; [ now eauto |].
+          intros Heq. eapply n. 
+          eapply H7; try now constructor.
+          rewrite extend_gss. rewrite extend_gso; eassumption. 
+  Qed.
   
-Definition preord_env_P_inj P k f rho1 rho2 :=
-  forall x : var,
-    P x -> preord_var_env k rho1 rho2 x (f x).
+  Lemma preord_env_P_inj_def_funs_pre k rho1 rho2 B1 B1' B2 B2' f h h' e :
+    (* The IH *)
+    (forall m : nat,
+       m < k ->
+       forall (e1 e2 : exp) (rho1 rho2 : env) (f : var -> var),
+         injective f ->
+         Alpha_conv e1 e2 f ->
+         preord_env_P_inj (occurs_free e1) m f rho1 rho2 ->
+         preord_exp pr m (e1, rho1) (e2, rho2)) ->
+    construct_fundefs_injection f B1 B2 h ->
+    construct_fundefs_injection f B1' B2' h' ->
+    injective f ->
+    Alpha_conv_fundefs B1 B2 h'  ->
+    Alpha_conv_fundefs B1' B2' h' ->
+    preord_env_P_inj (occurs_free (Efun B1' e)) k f rho1 rho2 ->
+    preord_env_P_inj (Union _ (occurs_free (Efun B1' e)) (name_in_fundefs B1)) k h
+                     (def_funs B1' B1 rho1 rho1) (def_funs B2' B2 rho2 rho2).
+  Proof.
+    revert B1 rho1 rho2 B1' B2 B2' f h h' e.
+    induction k as [ k IH' ] using lt_wf_rec1.
+    induction B1; intros rho1 rho2 B1' B2 B2' f h h' e' IHe Hinj Hinj' Hinj'' Ha Ha' Hpre.
+    - inv Ha. simpl. subst. inv Hinj. eapply preord_env_P_inj_set. 
+      + eapply preord_env_P_inj_antimon. now eapply IHB1; eauto.
+        rewrite !Setminus_Union_distr, Setminus_Empty_set, Union_Empty_set_r.
+        eapply Included_Union_compat.
+        * eapply Setminus_Included. now apply Included_refl.
+        * eapply Subset_Setminus.
+      + rewrite preord_val_eq.
+        intros vs1 vs2 j t1 xs1 e1 rho1' Hlen Hf Hs.
+        edestruct Alpha_conv_fundefs_find_def
+          as [xs2 [e2 [f'' [Hf' [Hlen' [Hinj''' Ha'' ] ] ] ] ] ]; [ apply Ha' | | | ]; eauto.
+        now eapply construct_fundefs_injection_injective; eauto.
+        edestruct setlist_length2 as [rho2' Hs']; eauto.
+        exists t1. exists xs2. exists e2. exists rho2'. split; eauto.
+        split; [ now eauto |]. intros Hleq Hpre'.
+        eapply IHe; [| | eassumption |]. omega.
+        eapply construct_lst_injection_injective; eauto.
+        now eapply construct_fundefs_injection_injective; eauto.
+        eapply preord_env_P_inj_antimon.
+        * eapply preord_env_P_inj_setlist;
+          [ | eassumption | eassumption | now eauto | now eauto  ].
+          eapply IH'; eauto. intros. eapply IHe. omega. now eauto. now eauto.
+          eassumption.
+          eapply (preord_env_P_inj_monotonic _ k). omega.
+          now eauto.
+        * apply find_def_correct in Hf; eauto.
+          rewrite occurs_free_Efun.
+          eapply Included_trans.
+          eapply occurs_free_in_fun. eassumption. 
+          rewrite Union_sym. eapply Included_Union_compat; [| now apply Included_refl ].
+          rewrite Union_sym. eapply Included_Union_compat; [| now apply Included_refl ].
+          now apply Included_Union_l.
+      + eassumption.
+    - inv Ha. simpl. inv Hinj. eapply preord_env_P_inj_antimon. eassumption.
+      rewrite Union_Empty_set_l. now apply Included_refl.
+  Qed.
 
-Lemma Forall2_app {A B} (P : A -> B -> Prop) xs ys f :
-   Forall2 (fun x y => f x = y) xs ys ->
-   (forall x y, List.In x xs -> f x = y -> P x y) ->
-   Forall2 P xs ys. 
-Proof. 
-  intros Hall Hyp. induction Hall.
-  - constructor.
-  - constructor.
-    + eapply Hyp. now constructor. eassumption.
-    + eapply IHHall.
-      intros. eapply Hyp. now constructor 2.
-      eassumption. 
-Qed.
-
-Lemma construct_fundefs_injection_injective f B1 B2 f' :
-  construct_fundefs_injection f B1 B2 f' ->
-  injective f ->
-  injective f'. 
-Proof.
-  intros H1 H2. induction H1; eauto. 
-Qed.
-
-Lemma construct_lst_injection_injective f xs ys f' :
-  construct_lst_injection f xs ys f' ->
-  injective f ->
-  injective f'. 
-Proof.
-  intros H1 H2. induction H1; eauto. 
-Qed.
-
-Lemma preord_env_P_inj_set (P : Ensemble var) (rho1 rho2 : env) 
-      (k : nat)  f(x y : var) (v1 v2 : val) : 
-  preord_env_P_inj (Setminus var P (Singleton var x)) k f rho1 rho2 ->
-  preord_val k v1 v2 ->
-  injective (f {x ~> y}) ->
-  preord_env_P_inj P k (f {x ~> y}) (M.set x v1 rho1) (M.set y v2 rho2).
-Proof. 
-  intros Henv Hv Hinj z HP. unfold extend. 
-  destruct (Coqlib.peq z x) as [| Hneq] eqn:Heq'.
-  - subst. intros z Hget.
-    rewrite M.gss in Hget. inv Hget. eexists. rewrite M.gss; eauto.
-  - intros z' Hget. rewrite M.gso in Hget; eauto.
-    destruct (Coqlib.peq (f z) y).
-    + exfalso. eapply Hneq. eapply Hinj. now constructor.
-      now constructor. rewrite extend_gso; eauto.
-      rewrite extend_gss. eassumption.
-    + edestruct (Henv z); eauto.
-      constructor; eauto. intros Hc. inv Hc. congruence. 
-      eexists. rewrite M.gso; eauto. 
-Qed.
-
-Lemma preord_env_P_inj_antimon (P1 P2 : var -> Prop) (k : nat) (rho1 rho2 : env) f :
-  preord_env_P_inj P2 k f rho1 rho2 ->
-  Included var P1 P2 -> preord_env_P_inj P1 k f rho1 rho2.
-Proof.
-  intros Henv Hi x HP. eapply Henv. now apply Hi.
-Qed.
-
-Lemma preord_env_P_inj_monotonic :
-  forall P (k j : nat) (rho1 rho2 : env) f,
-    j <= k -> preord_env_P_inj P k f rho1 rho2 -> preord_env_P_inj P j f rho1 rho2.
-Proof.
-  intros P k j rho1 rho2 f Hleq Hpre x HP v Hget.
-  edestruct Hpre as [v2 [Heq Hpre2] ]; eauto.
-  eexists; split; eauto. eapply preord_val_monotonic; eauto.
-Qed.
-
-Instance preord_env_P_inj_proper  :
-  Proper (Same_set var ==> Logic.eq ==> Logic.eq ==> Logic.eq ==> Logic.eq ==> iff)
-         preord_env_P_inj.
-Proof.
-  intros s1 s2 [H1 H2]; split; intros Hpre;
-  eapply preord_env_P_inj_antimon; subst; eauto.
-Qed.
-
-Lemma Alpha_conv_fundefs_find_def B1 B2 f g t xs1 e1 :
-  Alpha_conv_fundefs B1 B2 f ->
-  find_def g B1 = Some (t, xs1, e1) ->
-  injective f ->
-  exists xs2 e2 f', 
-    find_def (f g) B2 = Some (t, xs2, e2) /\
-    length xs1 = length xs2 /\
-    construct_lst_injection f xs1 xs2 f' /\
-    Alpha_conv e1 e2 f'.
-Proof. 
-  intros Ha Hdef Hinj. induction Ha. 
-  - inv Hdef. 
-  - simpl in Hdef. subst. destruct (M.elt_eq g g0).
-    + subst. inv Hdef. exists xs', e'.
-      simpl. rewrite Coqlib.peq_true. eauto.
-    + edestruct IHHa as [xs2 [ e2 Ha' ] ]; eauto.
-      edestruct (Coqlib.peq (f g) (f g0)). 
-      * eapply Hinj in e0. subst. congruence. now constructor.
+  (** α-equivalence preserves semantics *)
+  Lemma Alpha_conv_correct k rho1 rho2 e1 e2 f :
+    injective f ->
+    Alpha_conv e1 e2 f ->
+    preord_env_P_inj (occurs_free e1) k f rho1 rho2 ->
+    preord_exp pr k (e1, rho1) (e2, rho2).
+  Proof. 
+    revert e1 e2 rho1 rho2 f.
+    induction k as [ k IH ] using lt_wf_rec1.
+    induction e1 using exp_ind'; intros e2 rho1 rho2 f Hinj Ha Henv; inv Ha.
+    - eapply preord_exp_const_compat; eauto; intros.
+      + eapply Forall2_app; [ eassumption |].
+        intros x y Hin Heq. specialize (Henv x).
+        rewrite Heq in Henv. eapply Henv.
         now constructor.
-      * do 2 eexists. simpl. rewrite Coqlib.peq_false; eauto.
-Qed.
-
-Lemma setlist_length2 (rho rho' rho1 : env) (xs1 xs2 : list var) (vs1 vs2 : list val) :
-  length xs1 = length xs2 ->
-  length vs1 = length vs2 ->
-  setlist xs1 vs1 rho = Some rho1 ->
-  exists rho2 : M.t val, setlist xs2 vs2 rho' = Some rho2.
-Proof. 
- revert xs2 vs1 vs2 rho1.
- induction xs1 as [| x xs1 IHxs ]; intros xs2 vs1 vs2 rho1 Hlen1 Hlen2 Hset.
- - inv Hset. destruct vs1; try discriminate. inv H0.
-   destruct vs2; try discriminate. destruct xs2; try discriminate.
-   eexists; simpl; eauto.
- - destruct xs2; try discriminate.
-   destruct vs1; try discriminate. destruct vs2; try discriminate.
-   inv Hlen1. inv Hlen2. simpl in Hset. 
-   destruct (setlist xs1 vs1 rho) eqn:Heq2; try discriminate. inv Hset.
-   edestruct IHxs as [vs2' Hset2]; try eassumption.
-   eexists. simpl; rewrite Hset2; eauto.
-Qed.
-
-Lemma preord_env_P_inj_setlist (P1 : var -> Prop) (rho1 rho2 rho1' rho2' : env)
-      (k : nat) (xs1 xs2 : list var) (vs1 vs2 : list val) f f':
-  preord_env_P_inj P1 k f rho1 rho2 ->
-  Forall2 (preord_val k) vs1 vs2 ->
-  construct_lst_injection f xs1 xs2 f' ->
-  setlist xs1 vs1 rho1 = Some rho1' ->
-  setlist xs2 vs2 rho2 = Some rho2' ->
-  preord_env_P_inj (Union _ P1 (FromList xs1)) k f' rho1' rho2'.
-Proof.
-  revert P1 rho1 rho2 rho1' rho2' xs2 vs1 vs2 f f'. induction xs1;
-  intros P1 rho1 rho2 rho1' rho2' xs2 vs1 vs2  f f' Hpre Hall Hinj Hset1 Hset2 x HP v Hget.
-  - inv Hinj. destruct vs1; try discriminate.
-    inv Hall. 
-    inv Hset1; inv Hset2. eapply Hpre; eauto.
-    inv HP; [ now eauto | now inv H ]. 
-  - destruct vs1; try discriminate. inv Hall. inv Hinj.
-    simpl in Hset1, Hset2. 
-    destruct (setlist xs1 vs1 rho1) eqn:Heq1;
-      destruct (setlist ys l' rho2) eqn:Heq2; try discriminate.
-    inv Hset1; inv Hset2. rewrite M.gsspec in Hget.
-    destruct (Coqlib.peq x a); subst.
-    + inv Hget. eexists. 
-      simpl. unfold extend. rewrite Coqlib.peq_true.
-      rewrite M.gss. eauto.
-    + edestruct IHxs1 as [v2 [Het' Hpre'] ]; eauto.
-      * inv HP; [ now left; eauto |].
-        rewrite FromList_cons in H. inv H.
-        inv H0. congruence. right; eauto.
-      * eexists. unfold extend. rewrite Coqlib.peq_false; [| now eauto ].
-        rewrite M.gso; [ now eauto |].
-        intros Heq. eapply n. 
-        eapply H7; try now constructor.
-        rewrite extend_gss. rewrite extend_gso; eassumption. 
-Qed.
- 
-Lemma preord_env_P_inj_def_funs_pre k rho1 rho2 B1 B1' B2 B2' f h h' e :
-  (* The IH *)
-  (forall m : nat,
-     m < k ->
-     forall (e1 e2 : exp) (rho1 rho2 : env) (f : var -> var),
-       injective f ->
-       Alpha_conv e1 e2 f ->
-       preord_env_P_inj (occurs_free e1) m f rho1 rho2 ->
-       preord_exp m (e1, rho1) (e2, rho2)) ->
-  construct_fundefs_injection f B1 B2 h ->
-  construct_fundefs_injection f B1' B2' h' ->
-  injective f ->
-  Alpha_conv_fundefs B1 B2 h'  ->
-  Alpha_conv_fundefs B1' B2' h' ->
-  preord_env_P_inj (occurs_free (Efun B1' e)) k f rho1 rho2 ->
-  preord_env_P_inj (Union _ (occurs_free (Efun B1' e)) (name_in_fundefs B1)) k h
-                   (def_funs B1' B1 rho1 rho1) (def_funs B2' B2 rho2 rho2).
-Proof.
-  revert B1 rho1 rho2 B1' B2 B2' f h h' e.
-  induction k as [ k IH' ] using lt_wf_rec1.
-  induction B1; intros rho1 rho2 B1' B2 B2' f h h' e' IHe Hinj Hinj' Hinj'' Ha Ha' Hpre.
-  - inv Ha. simpl. subst. inv Hinj. eapply preord_env_P_inj_set. 
-    + eapply preord_env_P_inj_antimon. now eapply IHB1; eauto.
-      rewrite !Setminus_Union_distr, Setminus_Empty_set, Union_Empty_set_r.
-      eapply Included_Union_compat.
-      * eapply Setminus_Included. now apply Included_refl.
-      * eapply Subset_Setminus.
-    + rewrite preord_val_eq.
-      intros vs1 vs2 j t1 xs1 e1 rho1' Hlen Hf Hs.
-      edestruct Alpha_conv_fundefs_find_def
-        as [xs2 [e2 [f'' [Hf' [Hlen' [Hinj''' Ha'' ] ] ] ] ] ]; [ apply Ha' | | | ]; eauto.
-      now eapply construct_fundefs_injection_injective; eauto.
-      edestruct setlist_length2 as [rho2' Hs']; eauto.
-      exists t1. exists xs2. exists e2. exists rho2'. split; eauto.
-      split; [ now eauto |]. intros Hleq Hpre'.
-      eapply IHe; [| | eassumption |]. omega.
-      eapply construct_lst_injection_injective; eauto.
-      now eapply construct_fundefs_injection_injective; eauto.
+      + eapply IHe1. eassumption. eassumption.
+        eapply preord_env_P_inj_set; [| | eassumption ]. 
+        eapply preord_env_P_inj_antimon; eauto.
+        rewrite occurs_free_Econstr. now apply Included_Union_r.
+        rewrite preord_val_eq. constructor; eauto using Forall2_Forall2_asym_included.
+    - inv H1. eapply preord_exp_case_nil_compat.
+    - inv H1. destruct H2 as [Heq Ha]. destruct y as [c' e2]. simpl in Heq; subst.
+      eapply preord_exp_case_cons_compat; eauto.
+      eapply IHe1. eassumption. eassumption.
       eapply preord_env_P_inj_antimon.
-      * eapply preord_env_P_inj_setlist;
-        [ | eassumption | eassumption | now eauto | now eauto  ].
-        eapply IH'; eauto. intros. eapply IHe. omega. now eauto. now eauto.
-        eassumption.
-        eapply (preord_env_P_inj_monotonic _ k). omega.
-        now eauto.
-      * apply find_def_correct in Hf; eauto.
-        rewrite occurs_free_Efun.
-        eapply Included_trans.
-        eapply occurs_free_in_fun. eassumption. 
-        rewrite Union_sym. eapply Included_Union_compat; [| now apply Included_refl ].
-        rewrite Union_sym. eapply Included_Union_compat; [| now apply Included_refl ].
-        now apply Included_Union_l.
-    + eassumption.
-  - inv Ha. simpl. inv Hinj. eapply preord_env_P_inj_antimon. eassumption.
-    rewrite Union_Empty_set_l. now apply Included_refl.
-Qed.
+      eassumption. rewrite occurs_free_Ecase_cons. now apply Included_Union_l.
+      eapply IHe0. eassumption. now constructor; eauto.
+      eapply preord_env_P_inj_antimon.
+      eassumption. rewrite occurs_free_Ecase_cons.
+      rewrite Union_assoc. now apply Included_Union_r.
+    - eapply preord_exp_proj_compat; eauto; intros.
+      eapply IHe1. eassumption. eassumption.
+      eapply preord_env_P_inj_set; [| | eassumption ]. 
+      eapply preord_env_P_inj_antimon; eauto.
+      rewrite occurs_free_Eproj. now apply Included_Union_r. eassumption.
+    - eapply preord_exp_fun_compat; eauto.
+      eapply IHe1; [| eassumption |].
+      eapply construct_fundefs_injection_injective. eassumption. eassumption.
+      eapply preord_env_P_inj_antimon.
+      + eapply preord_env_P_inj_def_funs_pre; eauto.
+      + eapply occurs_free_Efun_Included.
+    - eapply preord_exp_app_compat.
+      + now eauto.
+      + eapply Forall2_app; [ eassumption |].
+        intros x y Hin Heq. specialize (Henv x).
+        rewrite Heq in Henv. eapply Henv.
+        now constructor.
+    - eapply preord_exp_prim_compat; eauto; intros.
+      + eapply Forall2_app; [ eassumption |].
+        intros x y Hin Heq. specialize (Henv x).
+        rewrite Heq in Henv. eapply Henv.
+        now constructor.
+      + eapply IHe1. eassumption. eassumption.
+        eapply preord_env_P_inj_set; [| | eassumption ]. 
+        eapply preord_env_P_inj_antimon; eauto.
+        rewrite occurs_free_Eprim. now apply Included_Union_r.
+        eauto. 
+  Qed.
 
-(** α-equivalence preserves semantics *)
-Lemma Alpha_conv_correct k rho1 rho2 e1 e2 f :
-  injective f ->
-  Alpha_conv e1 e2 f ->
-  preord_env_P_inj (occurs_free e1) k f rho1 rho2 ->
-  preord_exp k (e1, rho1) (e2, rho2).
-Proof. 
-  revert e1 e2 rho1 rho2 f.
-  induction k as [ k IH ] using lt_wf_rec1.
-  induction e1 using exp_ind'; intros e2 rho1 rho2 f Hinj Ha Henv; inv Ha.
-  - eapply preord_exp_const_compat; eauto; intros.
-    + eapply Forall2_app; [ eassumption |].
-      intros x y Hin Heq. specialize (Henv x).
-      rewrite Heq in Henv. eapply Henv.
-      now constructor.
-    + eapply IHe1. eassumption. eassumption.
-      eapply preord_env_P_inj_set; [| | eassumption ]. 
-      eapply preord_env_P_inj_antimon; eauto.
-      rewrite occurs_free_Econstr. now apply Included_Union_r.
-      rewrite preord_val_eq. constructor; eauto using Forall2_Forall2_asym_included.
-  - inv H1. eapply preord_exp_case_nil_compat.
-  - inv H1. destruct H2 as [Heq Ha]. destruct y as [c' e2]. simpl in Heq; subst.
-    eapply preord_exp_case_cons_compat; eauto.
-    eapply IHe1. eassumption. eassumption.
-    eapply preord_env_P_inj_antimon.
-    eassumption. rewrite occurs_free_Ecase_cons. now apply Included_Union_l.
-    eapply IHe0. eassumption. now constructor; eauto.
-    eapply preord_env_P_inj_antimon.
-    eassumption. rewrite occurs_free_Ecase_cons.
-    rewrite Union_assoc. now apply Included_Union_r.
-  - eapply preord_exp_proj_compat; eauto; intros.
-    eapply IHe1. eassumption. eassumption.
-    eapply preord_env_P_inj_set; [| | eassumption ]. 
-    eapply preord_env_P_inj_antimon; eauto.
-    rewrite occurs_free_Eproj. now apply Included_Union_r. eassumption.
-  - eapply preord_exp_fun_compat; eauto.
-    eapply IHe1; [| eassumption |].
-    eapply construct_fundefs_injection_injective. eassumption. eassumption.
-    eapply preord_env_P_inj_antimon.
-    + eapply preord_env_P_inj_def_funs_pre; eauto.
-    + eapply occurs_free_Efun_Included.
-  - eapply preord_exp_app_compat.
-    + now eauto.
-    + eapply Forall2_app; [ eassumption |].
-      intros x y Hin Heq. specialize (Henv x).
-      rewrite Heq in Henv. eapply Henv.
-      now constructor.
-  - eapply preord_exp_prim_compat; eauto; intros.
-    + eapply Forall2_app; [ eassumption |].
-      intros x y Hin Heq. specialize (Henv x).
-      rewrite Heq in Henv. eapply Henv.
-      now constructor.
-    + eapply IHe1. eassumption. eassumption.
-      eapply preord_env_P_inj_set; [| | eassumption ]. 
-      eapply preord_env_P_inj_antimon; eauto.
-      rewrite occurs_free_Eprim. now apply Included_Union_r.
-      eauto. 
-Qed.
+End Alpha_conv_correct.
 
 Close Scope fun_scope.
 Close Scope ctx_scope.
