theories/L6_PCPS/README.md
@@ -1,0 +1,72 @@
+# Description of the L6_PCPS directory
+
+### cps.v
+The syntax of the L6 language.
+
+### eval.v
+The evaluation semantics of the L6 language. 
+  
+### cps_util.v
+Useful lemmas and definitions about the L6 language.
+ 
+(TODO: Once we semantics are updated, we should clean-up a bit these three files) 
+
+### identifiers.v
+Definitions and lemmas about identifiers in L6. Among others, it contains
+formalizations of free variables, bound variables, unique bindings, and useful
+lemmas about them.
+
+### logical_relations.v
+Step-indexed logical relations. They are used in the correctness proofs of
+function hoisting and closure conversion.
+
+### L5_to_L6.v
+Translation from L5 to L6.
+
+### shrink_cps.v
+Shrink reduction.
+
+### uncurry.v  
+Uncurrying transformation for the L6 language.
+
+### closure_conversion.v
+Relational and computational definitions of closure conversion.
+
+### closure_conversion_correct.v
+Semantics preservation for the closure conversion relation.
+
+### closure_conversion_corresp.v
+Correspondence of the relational and computational definitions of closure
+conversion.
+
+### hoisting.v
+Function hoisting (relational and computational definition), correspondence of
+the two definitions and semantics preservation proof.
+
+### cps_show.v
+Pretty printer for the L6 language.
+
+### alpha_conv.v
+Formalization of alpha equivalence and semantics preservation proof.
+
+### ctx_approx.v
+Definition of of contextual approximation and equivalence. Proof that one of the
+logical relations is sound w.r.t. contextual approximation.
+
+### env.v
+Formalization of well-scopedness. (Maybe change the name of the file?)
+
+  
+## General libraries (not L6 related. Maybe move them to an other directory?)
+
+### hoare.v
+Hoare triples definitions and lemmas to reason about the state monad.
+### Ensembles_Util.v
+Useful definitions and lemmas about ensembles.
+### List_util.v
+Useful definitions and lemmas about lists.
+### set_util.v
+Useful definitions and lemmas about red-black sets (MSetRBT).
+### functions.v
+Useful definitions and lemmas about functions (extensional equality, image,
+codomain, injectivity, etc.).
